refocusing_lang_facts.v
@@ -1,0 +1,97 @@
+Require Export refocusing_lang.
+Require Import Program.
+Require Import Eqdep.
+
+Module RED_LANG_Facts (R : RED_LANG).
+
+    Import R.
+
+    Lemma ccons_inj : 
+        forall ec {k1 k2} (c : context k1 k2) ec' {k2'} (c' : context k1 k2'), 
+            k2 +> ec = k2' +> ec' -> ec=:c ~= ec'=:c' ->
+            ec = ec' /\ k2 = k2' /\ c ~= c'.
+    Proof.
+    intros.
+    assert (H1 := JMeq_eq_depT _ _ _ _ _ _ H H0).
+    assert (H2 := eq_dep_eq_sigT _ _ _ _ _ _ H1). 
+    inversion H2; subst.
+    assert (H7' := inj_pair2 _ _ _ _ _ H7); subst; clear H7.
+    assert (H7'' := inj_pair2 _ _ _ _ _ H7'); subst; clear H7'.
+    auto.
+    Qed.
+
+    Lemma context_tail_liveness : 
+        forall k ec, ~ dead_ckind (k+>ec) -> ~ dead_ckind k.
+    Proof.
+    intuition.
+    apply H.
+    apply ckind_death_propagation.
+    assumption.
+    Qed.
+
+    Lemma proper_death2 : forall k1 k2, context k1 k2 -> redex k2 -> ~ dead_ckind k1.
+    Proof.
+    intuition.
+    eapply proper_death;
+    eauto.
+    Qed.
+
+    Ltac inversion_ccons H :=
+
+      match type of H with ?ec1 =: ?c1  ~=  ?ec2 =: ?c2 => 
+
+      let H0 := fresh in 
+      assert (H0 : eq_dep _ _ _ (ec1=:c1) _ (ec2=:c2));
+
+      [ apply JMeq_eq_depT; eauto
+
+      | inversion H0; subst; 
+        match goal with H1 : existT _ _ _ = existT _ _ _ |- _ => 
+        let tmp := fresh in 
+        assert (tmp := H1); clear H1;
+        dependent destruction tmp
+        end;
+        clear H0 ]
+
+      end.
+
+  Lemma plug_empty    : forall t k, plug t (@empty k) = t.
+  Proof.
+  intuition.
+  Qed.
+
+  Lemma compose_empty : forall {k1 k2} (c : context k1 k2), c = c ~+ [_].
+  Proof.
+  induction c.
+  - trivial.
+  - simpl; rewrite <- IHc; trivial.
+  Qed.
+
+  Lemma plug_compose  : 
+      forall {k1 k2 k3} (c0 : context k1 k2) (c1 : context k3 k1) t, 
+           plug t (c0 ~+ c1) = plug (plug t c0) c1.
+  Proof.
+  induction c0; intros.
+  - trivial.
+  - simpl; rewrite IHc0; trivial.
+  Qed.
+
+  Lemma context_snoc : forall ec0 {k1 k2} (c0 : context k1 k2),
+                           exists ec1 c1, (ec0=:c0) = (c1~+ec1=:[_]).
+  Proof.
+  intros; revert ec0.
+  induction c0; intros.
+  - exists ec0; eexists [_]; trivial.
+  - destruct IHc0 with ec as (ec1, (c1, IH)).
+    exists ec1; eexists (ec0=:c1); rewrite IH; trivial.
+  Qed.
+
+  Lemma dead_contex_dead : forall {k1 k2}, context k1 k2 -> dead_ckind k1 -> dead_ckind k2.
+  Proof with auto.
+  intros ? ? c H; revert c.
+  induction 1.
+  - trivial.
+  - apply ckind_death_propagation...
+  Qed.
+
+End RED_LANG_Facts.
