refocusing_signatures.v
@@ -1,106 +1,108 @@
 Require Export refocusing_lang.
+Require Import Program.
+
 
 Module Type RED_SEM (R : RED_LANG).
 
-  Parameter dec : R.term -> forall {k1 k2}, R.context k1 k2 -> R.decomp k1 -> Prop.
+  Import R.
+
+  Parameter dec : term -> forall {k1 k2}, context k1 k2 -> decomp k1 -> Prop.
 
   (** A redex in context will only ever be reduced to itself *)
-  Axiom dec_redex_self : forall {k1 k2} (r : R.redex k2) (c : R.context k1 k2), 
-                             dec (R.redex_to_term r) c (R.d_red r c).
+  Axiom dec_redex_self : forall {k2} (r : redex k2) {k1} (c : context k1 k2), 
+                             dec r c (d_red r c).
 
-  Import R.
-  Axiom decompose : forall (t : R.term) k1, ~ R.dead_ckind k1 ->
-      (exists (v : R.value k1), t = R.value_to_term v) \/
-      (exists k2 (r : R.redex k2) (c : R.context k1 k2), R.plug (R.redex_to_term r) c = t).
+  Axiom decompose : forall (t : term) k1, ~ dead_ckind k1 ->
+      (exists (v : value k1), t = v) \/
+      (exists k2 (r : redex k2) (c : context k1 k2), plug r c = t).
 
   (** dec is left inverse of plug *)
-  Axiom dec_correct : forall t k1 k2 (c : R.context k1 k2) d, dec t c d -> 
-                          R.decomp_to_term d = R.plug t c.
+  Axiom dec_correct  : forall t {k1 k2} (c : context k1 k2) d, dec t c d -> 
+                           decomp_to_term d = plug t c.
 
-  Import R.
-  Axiom dec_plug     : forall k1 k2 (c : R.context k1 k2) k3 (c0 : R.context k3 k1) t d, 
-                          ~ dead_ckind k2 -> dec (R.plug t c) c0 d -> 
-                          dec t (R.compose c c0) d.
-  Axiom dec_plug_rev : forall k1 k2 (c : R.context k1 k2) k3 (c0 : R.context k3 k1) t d, 
-                          ~ dead_ckind k2 ->  dec t (R.compose c c0) d -> 
-                          dec (R.plug t c) c0 d.
+  Axiom dec_plug     : forall {k1 k2} (c : context k1 k2) {k3} (c0 : context k3 k1) t d, 
+                           ~ dead_ckind k2 -> dec (plug t c) c0 d -> 
+                           dec t (c ~+ c0) d.
 
-  Inductive decempty : R.term -> forall {k}, R.decomp k -> Prop :=
-  | d_intro : forall (t : R.term) {k} (d : R.decomp k), dec t (@R.empty k) d -> decempty t d.
+  Axiom dec_plug_rev : forall {k1 k2} (c : context k1 k2) {k3} (c0 : context k3 k1) t d, 
+                           ~ dead_ckind k2 ->  dec t (c ~+ c0) d -> 
+                           dec (plug t c) c0 d.
 
-  Inductive iter : forall {k}, R.decomp k -> R.value k -> Prop :=
-  | i_val : forall {k} (v : R.value k), iter (R.d_val v) v
-  | i_red : forall {k} (r : R.redex k) t {k'} (c : R.context k' k) d v,
-              R.contract r = Some t -> decempty (R.plug t c) d -> iter d v ->
-              iter (R.d_red r c) v.
+  Inductive decempty : term -> forall {k}, decomp k -> Prop :=
+  | d_intro : forall t {k} (d : decomp k), dec t [_] d -> decempty t d.
 
-  Inductive eval : R.term -> forall {k}, R.value k -> Prop :=
-  | e_intro : forall t {k} (d : R.decomp k) v, decempty t d -> iter d v -> eval t v.
+  Inductive iter : forall {k}, decomp k -> value k -> Prop :=
+  | i_val : forall {k} (v : value k), iter (d_val v) v
+  | i_red : forall {k2} (r : redex k2) t {k1} (c : context k1 k2) d v,
+              contract r = Some t -> decempty (plug t c) d -> iter d v ->
+              iter (d_red r c) v.
+
+  Inductive eval : term -> forall {k}, value k -> Prop :=
+  | e_intro : forall t {k} (d : decomp k) v, decempty t d -> iter d v -> eval t v.
 
 End RED_SEM.
 
+
 Module Type RED_REF_SEM (R : RED_LANG).
 
-  Import R.
+  Import R. 
 
   (** Functions specifying atomic steps of induction on terms and contexts -- needed to avoid explicit induction on terms and contexts in construction of the AM *)
-  Parameter dec_term    : R.term -> forall k, R.interm_dec k.
-  Parameter dec_context : forall (ec : R.elem_context) (k : R.ckind),
-                              R.value (R.ckind_trans k ec) -> R.interm_dec k.
+  Parameter dec_term    : term -> forall k, interm_dec k.
+  Parameter dec_context : forall ec k, value (k+>ec) -> interm_dec k.
 
 
   (*Axiom dec_term_liveness : 
-      forall t k, ~ R.dead_ckind k -> 
-      forall t0 ec0, dec_term t k = R.in_term t0 ec0 ->
-      ~ R.dead_ckind (R.ckind_trans k ec0).*)
+      forall t k, ~ dead_ckind k -> 
+      forall t0 ec0, dec_term t k = in_term t0 ec0 ->
+      ~ dead_ckind (ckind_trans k ec0).*)
 
   Axiom dec_term_correct : forall t k, match dec_term t k with
-    | R.in_red r => R.redex_to_term r = t
-    | R.in_val v => R.value_to_term v = t
-    | R.in_term t0 ec0 => R.atom_plug t0 ec0 = t
-    | R.in_dead => R.dead_ckind k
+    | in_red r => redex_to_term r = t
+    | in_val v => value_to_term v = t
+    | in_term t0 ec0 => atom_plug t0 ec0 = t
+    | in_dead => dead_ckind k
   end.
   Axiom dec_context_correct : forall ec k v, match dec_context ec k v with
-    | R.in_red r => R.redex_to_term r = R.atom_plug (R.value_to_term v) ec
-    | R.in_val v0 => R.value_to_term v0 = R.atom_plug (R.value_to_term v) ec
-    | R.in_term t ec0 => R.atom_plug t ec0 = R.atom_plug (R.value_to_term v) ec
-    | R.in_dead => R.dead_ckind (R.ckind_trans k ec) 
+    | in_red r => redex_to_term r = atom_plug (value_to_term v) ec
+    | in_val v0 => value_to_term v0 = atom_plug (value_to_term v) ec
+    | in_term t ec0 => atom_plug t ec0 = atom_plug (value_to_term v) ec
+    | in_dead => dead_ckind (k+>ec) 
   end.
 
   (** A decomposition function specified in terms of the atomic functions above *)
-  Inductive dec : R.term -> forall {k1 k2}, R.context k1 k2 -> R.decomp k1 -> Prop :=
-  | d_dec  : forall t {k1 k2} (c : R.context k1 k2) (r : R.redex k2),
-               dec_term t k2 = R.in_red r -> 
-               dec t c (R.d_red r c)
-  | d_v    : forall t {k1 k2} (c : R.context k1 k2) (v : R.value k2) (d : R.decomp k1),
-               dec_term t k2 = R.in_val v ->
+  Inductive dec : term -> forall {k1 k2}, context k1 k2 -> decomp k1 -> Prop :=
+  | d_dec  : forall t {k1 k2} (c : context k1 k2) r,
+               dec_term t k2 = in_red r -> 
+               dec t c (d_red r c)
+  | d_v    : forall t {k1 k2} (c : context k1 k2) v d,
+               dec_term t k2 = in_val v ->
                decctx v c d ->
                dec t c d
-  | d_term : forall t t0 {k1 k2} (c : R.context k1 k2) ec (d : R.decomp k1),
-               dec_term t k2 = R.in_term t0 ec ->
-               dec t0 (R.ccons ec c) d ->
+  | d_term : forall t t0 {k1 k2} (c : context k1 k2) ec d,
+               dec_term t k2 = in_term t0 ec ->
+               dec t0 (ccons ec c) d ->
                dec t c d
-  with decctx : forall {k2}, R.value k2 -> forall {k1}, R.context k1 k2 -> R.decomp k1 -> Prop :=
-  | dc_end  : forall {k} (v : R.value k), 
-                ~ R.dead_ckind k ->
-                decctx v (@R.empty k) (R.d_val v)
-  | dc_dec  : forall ec {k2} (v : R.value (R.ckind_trans k2 ec)) 
-                        {k1} (c : R.context k1 k2) (r : R.redex k2),
-                dec_context ec k2 v = R.in_red r ->
-                decctx v (R.ccons ec c) (R.d_red r c)
-  | dc_val  : forall {k2} (v0 : R.value k2) ec   (v : R.value (R.ckind_trans k2 ec)) 
-                     {k1} (c  : R.context k1 k2) (d : R.decomp k1),
-                dec_context ec k2 v = R.in_val v0 ->
+  with decctx : forall {k2}, value k2 -> forall {k1}, context k1 k2 -> decomp k1 -> Prop :=
+  | dc_end  : forall {k} (v : value k), 
+                ~ dead_ckind k ->
+                decctx v [_] (d_val v)
+  | dc_dec  : forall ec {k2} (v : value (k2+>ec)) {k1} (c : context k1 k2) r,
+                dec_context ec k2 v = in_red r ->
+                decctx v (ccons ec c) (d_red r c)
+  | dc_val  : forall {k2} (v0 : value k2) ec (v : value (k2+>ec)) 
+                     {k1} (c  : context k1 k2) d,
+                dec_context ec k2 v = in_val v0 ->
                 decctx v0 c d ->
-                decctx v (R.ccons ec c) d
-  | dc_term : forall ec ec0 {k2} (v : R.value (R.ckind_trans k2 ec)) 
-                            {k1} (c : R.context k1 k2) (t : R.term) (d : R.decomp k1),
-                dec_context ec k2 v = R.in_term t ec0 ->
-                dec t (R.ccons ec0 c) d ->
-                decctx v (R.ccons ec c) d.
+                decctx v (ccons ec c) d
+  | dc_term : forall ec ec0 {k2} (v : value (k2+>ec)) 
+                            {k1} (c : context k1 k2) t d,
+                dec_context ec k2 v = in_term t ec0 ->
+                dec t (ccons ec0 c) d ->
+                decctx v (ccons ec c) d.
 
-  Axiom dec_val_self : forall k2 (v : R.value k2) k1 (c : R.context k1 k2) (d : R.decomp k1), 
-                           dec (R.value_to_term v) c d <-> decctx v c d.
+  Axiom dec_val_self : forall {k2} (v : value k2) {k1} (c : context k1 k2) d, 
+                           dec (value_to_term v) c d <-> decctx v c d.
 
   Declare Module RS : RED_SEM R with Definition dec := dec.
 
@@ -109,37 +111,43 @@ Module Type RED_REF_SEM (R : RED_LANG).
 
 End RED_REF_SEM.
 
-
+(*
 Module Type PE_REF_SEM (R : RED_LANG).
+
+  Import R.
 
   Declare Module Red_Sem : RED_REF_SEM R.
 
-  Axiom dec_context_not_val : forall k (v0 : R.value k) (ec : R.elem_context) 
-                                       (v  : R.value (R.ckind_trans k ec)), 
-            Red_Sem.dec_context ec k v <> R.in_val v0.
-  Import R.
+  Axiom dec_context_not_val : forall k v0 ec v, 
+            Red_Sem.dec_context ec k v <> in_val v0.
   Axiom dec_term_value : forall k v, 
-                             Red_Sem.dec_term (R.value_to_term v) k = R.in_val v.
+                             Red_Sem.dec_term (value_to_term v) k = in_val v.
 
-End PE_REF_SEM.
+End PE_REF_SEM.*)
 
-Require Import Program.
 
-Module Type RED_PROP (R : RED_LANG) (RS : RED_REF_SEM(R)).
+Module Type RED_PROP (R : RED_LANG) (RS : RED_SEM(R)).
 
-  Axiom dec_is_function  : forall t k (d d0 : R.decomp k), 
-                               RS.RS.decempty t d -> RS.RS.decempty t d0 -> d = d0.
-  Axiom iter_is_function : forall k d (v v0 : R.value k), 
-                               RS.RS.iter d v -> RS.RS.iter d v0 -> v = v0.
-  Axiom eval_is_function : forall t k (v v0 : R.value k), 
-                               RS.RS.eval t v -> RS.RS.eval t v0 -> v = v0.
-  Axiom dec_correct : forall t k1 k2 (c : R.context k1 k2) d, 
-                          RS.RS.dec t c d -> R.decomp_to_term d = R.plug t c.
-  Axiom dec_total : forall t k, ~ R.dead_ckind k -> exists (d : R.decomp k), RS.RS.decempty t d.
-  Axiom unique_decomposition : forall t k, ~ R.dead_ckind k ->  
-      (exists v : R.value k, t = R.value_to_term v) \/ 
-      (exists k2 (r : R.redex k2) (c : R.context k k2),  R.plug (R.redex_to_term r) c = t /\ 
-	  forall k2' (r0 : R.redex k2') (c0 : R.context k k2'), 
-              R.plug (R.redex_to_term r0) c0 = t -> k2' = k2 /\ r ~= r0 /\ c ~= c0).
+  Import R.
+  Import RS.
+
+  Axiom dec_is_function  : forall t {k} (d d0 : decomp k), 
+                               decempty t d -> decempty t d0 -> d = d0.
+  Axiom iter_is_function : forall {k} (d : decomp k) v v0, 
+                               iter d v -> iter d v0 -> v = v0.
+  Axiom eval_is_function : forall t {k} (v v0 : value k), 
+                               eval t v -> eval t v0 -> v = v0.
+  Axiom dec_correct      : forall t {k1 k2} (c : context k1 k2) d,
+                               dec t c d -> decomp_to_term d = plug t c.
+  Axiom dec_total        : forall t k, ~ dead_ckind k -> 
+                               exists (d : decomp k), decempty t d.
+  Axiom unique_decomposition : 
+      forall t k1, ~ dead_ckind k1 ->  
+
+         (exists v : R.value k1, value_to_term v = t) \/
+
+         (exists k2 (r : redex k2) (c : context k1 k2), plug r c = t /\ 
+	      forall k2' (r' : redex k2') (c' : context k1 k2'), 
+                  plug r' c' = t -> k2' = k2 /\ r ~= r' /\ c ~= c').
 
 End RED_PROP.
